C0deine/Experimental/Prover/Interface.lean
@@ -1,0 +1,32 @@
+/- C0deine - Prover.Interface
+   Components that interface with the compiler frontend
+   - Thea Brick
+ -/
+import C0deine.Top
+-- import C0deine.Type.SyntaxTree.Dynamics
+-- import C0deine.Type.SyntaxTree.Dynamics.Notation
+-- import C0deine.Type.SyntaxTree.Dynamics.Transitivity
+-- import C0deine.Experimental.Prover.Tactics
+
+namespace C0deine.Prover
+
+open Top
+
+def parse_tc (prog : String) : Option (Tst.Prog × Context.State) := do
+  -- let libSearchDirs ← mkLibSearchDirs [] []
+  let config : Config := default
+    -- { (default : Config) with libSearchDirs := libSearchDirs }
+  let  (tst, _config, ctx) ← runFrontendNoIO config prog
+  return (tst, ctx)
+
+def parse_tc! (prog : String) : Tst.Prog × Context.State :=
+  match parse_tc prog with
+  | none => panic! "Could not typecheck program!"
+  | some res => res
+
+
+def verify (prog_ctx : Tst.Prog × Context.State) (func : String) := do
+  let (prog, ctx) := prog_ctx
+  let fdef ← prog.findFuncDef (ctx.symbolCache.find! func)
+  return ()
+
