C0deine/Experimental/Prover/Playground.lean
@@ -1,0 +1,31 @@
+/- C0deine - Prover.Playground
+   Testing area for verifying C0 code
+   - Thea Brick
+ -/
+import C0deine.Experimental.Prover.Interface
+import C0deine.Experimental.Prover.Tactics
+
+namespace C0deine.Prover.Playground
+
+def prog₁ := parse_tc! "
+int main() {
+  int x = 150;
+  //@assert x == 150;
+  return 150;
+}"
+
+#eval verify prog₁ "main"
+
+
+open Typ.Notation in
+def tst : Tst.Expr {} {} (int) :=
+  Tst.Expr.binop_int (by rfl) (by rfl) (by rfl)
+    .plus (.num (by rfl) 5) (.num (by rfl) 5)
+
+open Tst.Dynamics Notation in
+example /-  5 + 5 ==>* 10   -/
+       : (H; S; η |= (.eval tst .nil)                       [prog|p])
+    ==>* (H; S; η |= (.val (Δ:={}) (Γ:={}) (.num 10) .nil)  [prog|p])
+    := by
+  rw [tst]
+  repeat c0_step
